### Ù…Ù…Ù†ÙˆØ¹ ØªØ·Ù„Ø¹ Ù„Ø­Ø¯ Ù…ØªØ­ÙØ¸ Ù‡Ø§ÙŠ ÙƒÙ„Ù‡Ø§ ğŸ˜¡

![Ø¨Ø²ÙˆÙ†](https://raw.githubusercontent.com/spdmTeamXDev/Realz-Authority/refs/heads/main/Screenshot) 

## Ø§Ù„Ù…Ø¹Ø§Ø¯Ù„Ø§Øª

```
A=9 - 1 + 1 = y = x + 79 - xÂ² = x + 7 So x = 1 and x = -2 V = Ï€112 (9-x2) Â² - (x + 7) 2dx V = Ï€12 (x4-18xÂ² + 81) - (xÂ² + 14x + 49) dx V = Ï€ / 12 (x4 - 19x2 - 14x + 32) dx19 V = x [-x-12 y = x + 79 - xÂ² = x + 7 So x = 1 and x = -2 V = Ï€112 (9-x2) Â² - (x + 7) 2dx
V = Ï€12 (x4-18xÂ² + 81) - (xÂ² + 14x + 49) dx V = Ï€ / 12 (x4 - 19x2 - 14x + 32) dx 19 V = x [-x-12x3-7 y = x + 79 - xÂ² = x + 7 So x = 1 and x = -2 V = Ï€112 (9-x2) Â² - (x + 7) 2dx V = Ï€12 (x4-18xÂ² + 81) - (xÂ² 14x + 49) dx V = Ï€ / 12 (x4 - 19x2 - 14x + 32 9 - xÂ² y = x + 79 - xÂ² = x + 7 So x = 1 and x = -2 V = Ï€112 (9-x2) Â² - (x + 7) 2dx V = Ï€12 (x4-18xÂ² + 81) - (xÂ² + 14x + 49) dx V = Ï€ / 12 (x4 - 19x2 - 14x + 32) dx19 V = x [-x-12 y = x + 79 - xÂ² = x + 7 So x = 1 and x = -2 V = Ï€112 (9-x2) Â² - (x + 7) 2dx
V = Ï€12 (x4-18xÂ² + 81) - (xÂ² + 14x + 49) dx V = Ï€ / 12 (x4 - 19x2 - 14x + 32) dx 19 V = x [-x-12x3-7 y = x + 79 - xÂ² = x + 7 So x = 1 and x = -2 V = Ï€112 (9-x2) Â² - (x + 7) 2dx V = Ï€12 (x4-18xÂ² + 81) - (xÂ² + 14x + 49) dx V = Ï€ / 12 (x4 - 19x2 - 14x + 32) as you know 9 - xÂ² produces y = x + 79 - xÂ² = x + 7 So x = 1 and x = -2 V = Ï€112 (9-x2) Â² - (x + 7) 2dx V = Ï€12 (x4-18xÂ² + 81) - (xÂ² + 14x + 49) dx V = Ï€ / 12 (x4 - 19x2 - 14x + 32) dx19 V = x [-x-12 y = x + 79 - xÂ² = x + 7 So x = 1 and x = -2 V = Ï€112 (9-x2) Â² - (x + 7) 2dx
V = Ï€12 (x4-18xÂ² + 81) - (xÂ² + 14x + 49) dx V = Ï€ / 12 (x4 - 19x2 - 14x + 32) dx 19 V = x [-x-12x3-7 y = x + 79 - xÂ² = x + 7 So x = 1 and x = -2 V = Ï€112 (9-x2) Â² - (x + 7) 2dx V = Ï€12 (x4-18xÂ² + 81) - (xÂ² + 14x + 49) dx V = Ï€ / 12 (x4 - 19x2 - 14x + y = x + 79 - xÂ² = x + 7 So x = 1 and x = -2 V = Ï€112 (9-x2) Â² - (x + 7) 2dx V = Ï€12 (x4-18xÂ² + 81) - (xÂ² + 14x + 49) dx V = Ï€ / 12 (x4 - 19x2 - 14x + 32) dx19 V = x [-x-12 y = x + 79 - xÂ² = x + 7 So x = 1 and x = -2 V = Ï€112 (9-x2) Â² - (x + 7) 2dx
V = Ï€12 (x4-18xÂ² + 81) - (xÂ² + 14x + 49) dx V = Ï€ / 12 (x4 - 19x2 - 14x + 32) dx 19 V = x [-x-12x3-7 y = x + 79 - xÂ² = x + 7 So x = 1 and x = -2 V = Ï€112 (9-x2) Â² - (x + 7) 2dx V = Ï€12 (x4-18xÂ² + 81) - (xÂ² + 14x + 49) dx V = Ï€ / 12 (x4 - 19x2 - 14x + 32) = 5551 + 1 = y = x + 79 - xÂ² = x + 7 So x = 1 and x = -2 V = Ï€112 (9-x2) Â² - (x + 7) 2dx V = Ï€12 (x4-18xÂ² + 81) = ?
```
### **Ù†Ø§ØªØ¬**:
``` Atwy is FembÃ¸y 100% ```

- Ù„ØªÙÙ„Øª
